lib/zoo_std/random_round.ml
@@ -1,11 +1,11 @@
 type t =
-  { random: Random.t;
+  { random: Random_state.t;
     array: int array;
     mutable index: int;
   }
 
 let create sz =
-  { random= Random.create ();
+  { random= Random_state.create ();
     array= Array.unsafe_initi sz (fun i -> i);
     index= sz;
   }
@@ -16,7 +16,7 @@ let reset t =
 let next t =
   let arr = t.array in
   let i = t.index in
-  let j = Random.int t.random i in
+  let j = Random_state.int t.random i in
   let res = Array.unsafe_get arr j in
   let i = i - 1 in
   Array.unsafe_set arr j (Array.unsafe_get arr i) ;
