lib/zoo_std/random_state.mli
@@ -1,0 +1,12 @@
+type t
+
+val create :
+  unit -> t
+
+val bits :
+  t -> int
+
+val int :
+  t -> int -> int
+val int_in_range :
+  t -> int -> int -> int
