theories/zoo_std/random_round__code.v
@@ -4,8 +4,8 @@ From zoo.language Require Import
   typeclasses
   notations.
 From zoo_std Require Import
-  random
-  array.
+  array
+  random_state.
 From zoo_std Require Import
   random_round__types.
 From zoo Require Import
@@ -13,7 +13,10 @@ From zoo Require Import
 
 Definition random_round_create : val :=
   fun: "sz" =>
-    { random_create (), array_unsafe_initi "sz" (fun: "i" => "i"), "sz" }.
+    { random_state_create (),
+      array_unsafe_initi "sz" (fun: "i" => "i"),
+      "sz"
+    }.
 
 Definition random_round_reset : val :=
   fun: "t" =>
@@ -23,7 +26,7 @@ Definition random_round_next : val :=
   fun: "t" =>
     let: "arr" := "t".{array} in
     let: "i" := "t".{index} in
-    let: "j" := random_int "t".{random} "i" in
+    let: "j" := random_state_int "t".{random} "i" in
     let: "res" := array_unsafe_get "arr" "j" in
     let: "i" := "i" - #1 in
     array_unsafe_set "arr" "j" (array_unsafe_get "arr" "i") ;;
