theories/zoo_std/random_round__types.v
@@ -4,8 +4,8 @@ From zoo.language Require Import
   typeclasses
   notations.
 From zoo_std Require Import
-  random
-  array.
+  array
+  random_state.
 From zoo Require Import
   options.
 
