theories/zoo_std/random_state.v
@@ -1,0 +1,106 @@
+From zoo Require Import
+  prelude.
+From zoo.language Require Import
+  notations.
+From zoo.diaframe Require Import
+  diaframe.
+From zoo_std Require Export
+  base
+  random_state__code.
+From zoo Require Import
+  options.
+
+Implicit Types t : val.
+
+Parameter random_state_model : ∀ `{zoo_G : !ZooG Σ}, val → iProp Σ.
+
+Axiom random_state_create_spec : ∀ `{zoo_G : !ZooG Σ},
+  {{{
+    True
+  }}}
+    random_state_create ()
+  {{{ t,
+    RET t;
+    random_state_model t
+  }}}.
+
+Axiom random_state_bits_spec : ∀ `{zoo_G : !ZooG Σ} t,
+  {{{
+    random_state_model t
+  }}}
+    random_state_bits t
+  {{{ (n : Z),
+    RET #n;
+    random_state_model t
+  }}}.
+
+Axiom random_state_int_spec : ∀ `{zoo_G : !ZooG Σ} t ub,
+  (0 < ub)%Z →
+  {{{
+    random_state_model t
+  }}}
+    random_state_int t #ub
+  {{{ n,
+    RET #n;
+    ⌜0 ≤ n < ub⌝%Z ∗
+    random_state_model t
+  }}}.
+
+Section zoo_G.
+  Context `{zoo_G : !ZooG Σ}.
+
+  Lemma random_state_int_spec_nat t (ub : nat) :
+    0 < ub →
+    {{{
+      random_state_model t
+    }}}
+      random_state_int t #ub
+    {{{ n,
+      RET #n;
+      ⌜n < ub⌝ ∗
+      random_state_model t
+    }}}.
+  Proof.
+    iIntros "%Hub %Φ Ht HΦ".
+    wp_apply (random_state_int_spec with "Ht") as (n) "(%Hn & Ht)"; first lia.
+    Z_to_nat n. iSteps.
+  Qed.
+
+  Lemma random_state_int_in_range_spec t lb ub :
+    (lb < ub)%Z →
+    {{{
+      random_state_model t
+    }}}
+      random_state_int_in_range t #lb #ub
+    {{{ n,
+      RET #n;
+      ⌜lb ≤ n < ub⌝%Z ∗
+      random_state_model t
+    }}}.
+  Proof.
+    iIntros "%Hlt %Φ Ht HΦ".
+    wp_rec.
+    wp_smart_apply (random_state_int_spec with "Ht") as "%n (%Hn & Ht)"; first lia.
+    iSteps.
+  Qed.
+  Lemma random_state_int_in_range_spec_nat t lb ub :
+    lb < ub →
+    {{{
+      random_state_model t
+    }}}
+      random_state_int_in_range t #lb #ub
+    {{{ n,
+      RET #n;
+      ⌜lb ≤ n < ub⌝ ∗
+      random_state_model t
+    }}}.
+  Proof.
+    iIntros "%Hlt %Φ Ht HΦ".
+    wp_rec.
+    wp_smart_apply (random_state_int_spec with "Ht") as "%n (%Hn & Ht)"; first lia.
+    wp_pures.
+    Z_to_nat n. rewrite -Nat2Z.inj_add. iSteps.
+  Qed.
+End zoo_G.
+
+#[global] Opaque random_state_int_in_range.
