theories/zoo_std/random_state__code.v
@@ -1,0 +1,19 @@
+From zoo Require Import
+  prelude.
+From zoo.language Require Import
+  typeclasses
+  notations.
+From zoo_std Require Import
+  random_state__types.
+From zoo Require Import
+  options.
+
+Parameter random_state_create : val.
+
+Parameter random_state_bits : val.
+
+Parameter random_state_int : val.
+
+Definition random_state_int_in_range : val :=
+  fun: "t" "lb" "ub" =>
+    "lb" + random_state_int "t" ("ub" - "lb").
